changed quickSort to sort arbitrary arrays

sv_boogie.bpl
@@ -4,7 +4,9 @@ axiom 0 <= N;
 
 // Declare a map from integers to integers.
 // 'a' should be treated as an array of 'N' elements, indexed from 0 to N-1
-var a, b0, b1, b2: [int]int;
+var a: [int]int;
+// internal variable that is used by quicksort implementation
+var a_qs:  [int]int;
 
 // Returns true iff the elements of 'arr' are small (i.e. values in the range -3N to +3N)
 function has_small_elements(arr: [int]int): bool
@@ -14,7 +16,7 @@ function has_small_elements(arr: [int]int): bool
 
 // Sorts 'a' using bucket sort or quick sort, as determined by has_small_elements(a)
 procedure sort() returns (perm : [int]int)
-  modifies a,b0,b1,b2;
+  modifies a, a_qs;
   // perm is a permutation
   ensures (forall i: int :: 0 <= i && i <= N-1 ==> 0 <= perm[i] && perm[i] <= N-1);
   ensures (forall k, l: int :: 0 <= k && k < l && l <= N-1 ==> perm[k] != perm[l]);
@@ -29,29 +31,30 @@ procedure sort() returns (perm : [int]int)
     if (has_small_elements(a))
     {
         // sort 'a' using bucket sort
-        call perm := bs();
+        call perm := bucketSort(0,N-1);
     } else {
         // sort 'a' using quick sort
-        call perm := qs(0,N-1);
+        call a, perm := quickSort(a,0,N-1);
     }     
   }
  
 }
 
+
 procedure qsPartition(lo : int, hi : int) returns (pivot_index: int, perm: [int]int) 
-  modifies a;
+  modifies a_qs;
   requires lo <= hi;
   ensures lo <= pivot_index && pivot_index <= hi;
   // array is correctly partitioned
-  ensures (forall k: int :: lo <= k && k < pivot_index ==> a[k] <= a[pivot_index]);
-  ensures (forall k: int :: pivot_index < k && k <= hi ==> a[k] > a[pivot_index]);
+  ensures (forall k: int :: lo <= k && k < pivot_index ==> a_qs[k] <= a_qs[pivot_index]);
+  ensures (forall k: int :: pivot_index < k && k <= hi ==> a_qs[k] > a_qs[pivot_index]);
   // perm is a permutation
   ensures (forall i: int :: lo <= i && i <= hi ==> lo <= perm[i] && perm[i] <= hi);
   ensures (forall i, j: int :: lo <= i && i < j && j <= hi ==> perm[i] != perm[j]);
   // the final array is that permutation of the input array
-  ensures (forall i: int :: lo <= i && i <= hi ==> a[i] == old(a)[perm[i]]);
+  ensures (forall i: int :: lo <= i && i <= hi ==> a_qs[i] == old(a_qs)[perm[i]]);
   // only the indexes between lo and hi are modified, the rest of the array stays the same
-  ensures (forall i: int :: i < lo || i > hi ==> a[i] == old(a)[i]);
+  ensures (forall i: int :: i < lo || i > hi ==> a_qs[i] == old(a_qs)[i]);
 {
 
   // local variables
@@ -73,37 +76,37 @@ procedure qsPartition(lo : int, hi : int) returns (pivot_index: int, perm: [int]
   j := lo;
   
   
-  pivot := a[hi];
+  pivot := a_qs[hi];
   while(j < hi) 
-    invariant pivot == a[hi];
+    invariant pivot == a_qs[hi];
     invariant lo - 1 <= i && i < j && j <= hi;
  
     // correct partition
-    invariant (forall k: int :: lo <= k && k <= i ==> a[k] <= pivot);
-    invariant (forall k: int :: i < k && k < j ==> a[k] > pivot);
+    invariant (forall k: int :: lo <= k && k <= i ==> a_qs[k] <= pivot);
+    invariant (forall k: int :: i < k && k < j ==> a_qs[k] > pivot);
     
     // correct permutation
     invariant (forall k: int :: lo <= k && k <= hi ==> lo <= perm[k] && perm[k] <= hi);
     invariant (forall k, l: int :: lo <= k && k < l && l <= hi ==> perm[k] != perm[l]);
     
     // final array is permutation of original
-    invariant (forall k: int :: lo <= k && k <= hi ==> a[k] == old(a)[perm[k]]);
+    invariant (forall k: int :: lo <= k && k <= hi ==> a_qs[k] == old(a_qs)[perm[k]]);
     
     // rest of the array is untouched
-    invariant (forall k: int :: k < lo || k > hi ==> a[k] == old(a)[k]);
+    invariant (forall k: int :: k < lo || k > hi ==> a_qs[k] == old(a_qs)[k]);
     
   {
-    if(a[j] <= pivot) {
+    if(a_qs[j] <= pivot) {
       i := i + 1;
-      // swap a[i] with a[j]
-      tmp := a[i]; a[i] := a[j]; a[j] := tmp;
+      // swap a_qs[i] with a_qs[j]
+      tmp := a_qs[i]; a_qs[i] := a_qs[j]; a_qs[j] := tmp;
       tmp := perm[i]; perm[i] := perm[j]; perm[j] := tmp;
     }
     j := j + 1;
   }
   
-  //swap a[i+1] with a[hi], the pivot element
-  tmp := a[i+1];  a[i+1] := a[hi];  a[hi] := tmp;
+  //swap a_qs[i+1] with a_qs[hi], the pivot element
+  tmp := a_qs[i+1];  a_qs[i+1] := a_qs[hi];  a_qs[hi] := tmp;
   tmp := perm[i+1]; perm[i+1] := perm[hi]; perm[hi] := tmp;
   
   pivot_index := i+1;
@@ -112,20 +115,20 @@ procedure qsPartition(lo : int, hi : int) returns (pivot_index: int, perm: [int]
 
 
 procedure qs(lo : int, hi : int) returns (perm: [int]int) 
-  modifies a;
+  modifies a_qs;
   requires lo <= hi;
   
   // perm is a permutation
   ensures (forall i: int :: lo <= i && i <= hi ==> lo <= perm[i] && perm[i] <= hi);
   ensures (forall k, l: int :: lo <= k && k < l && l <= hi ==> perm[k] != perm[l]);
   // the final array is that permutation of the input array
-  ensures (forall i: int :: lo <= i && i <= hi ==> a[i] == old(a)[perm[i]]);
+  ensures (forall i: int :: lo <= i && i <= hi ==> a_qs[i] == old(a_qs)[perm[i]]);
   
   // array is sorted
-  ensures (forall k, l: int :: lo <= k && k <= l && l <= hi ==> a[k] <= a[l]);
+  ensures (forall k, l: int :: lo <= k && k <= l && l <= hi ==> a_qs[k] <= a_qs[l]);
   
   // rest of the array is untouched
-  ensures (forall k: int :: k < lo || k > hi ==> a[k] == old(a)[k]);
+  ensures (forall k: int :: k < lo || k > hi ==> a_qs[k] == old(a_qs)[k]);
 {
    // local variables
   var n, pivot_index: int;
@@ -161,17 +164,15 @@ procedure qs(lo : int, hi : int) returns (perm: [int]int)
     
     perm_comb[pivot_index] := pivot_index;
     // perm_comb is now a permutation
-    assert (forall i: int :: lo <= i && i <= hi ==> lo <= perm_comb[i] && perm_comb[i] <= hi);
-    assert (forall k, l: int :: lo <= k && k < l && l <= hi ==> perm_comb[k] != perm_comb[l]);
-    
-    // assert that perm combined with perm_comb is a permutation
+
+    // combine perm_comb with perm
     n := lo;
     while(n <= hi) 
       invariant lo <= n && n <= hi+1;
       invariant (forall i: int :: lo <= i && i < n ==> perm[i] == perm_comb[perm[i]]);
       invariant (forall i: int :: lo <= i && i < n ==> lo <= perm[i] && perm[i] <= hi);
       invariant (forall k, l: int :: lo <= k && k < l && l < n ==> perm[k] != perm[l]);
-      invariant (forall i: int :: lo <= i && i < n ==> a[i] == old(a)[perm[i]]);
+      invariant (forall i: int :: lo <= i && i < n ==> a_qs[i] == old(a_qs)[perm[i]]);
     { perm[n] := perm_comb[perm[n]]; }
     
   } else {
@@ -180,93 +181,39 @@ procedure qs(lo : int, hi : int) returns (perm: [int]int)
     
 }
 
-/*
-// dummy sort implementation for faster development times
-procedure qs(lo : int, hi : int) returns (perm: [int]int) 
-  modifies a;
+// public interface for quicksort that can be used to sort arbitrary arrays
+procedure quickSort(arr : [int]int, lo : int, hi : int) returns (arr_sorted : [int]int, perm: [int]int) 
+  modifies a_qs;
   requires lo <= hi;
-  
+  // perm is a permutation
+  ensures (forall i: int :: lo <= i && i <= hi ==> lo <= perm[i] && perm[i] <= hi);
+  ensures (forall k, l: int :: lo <= k && k < l && l <= hi ==> perm[k] != perm[l]);
+  // the final array is that permutation of the input array
+  ensures (forall i: int :: lo <= i && i <= hi ==> arr_sorted[i] == arr[perm[i]]);
+  // array is sorted
+  ensures (forall k, l: int :: lo <= k && k <= l && l <= hi ==> arr_sorted[k] <= arr_sorted[l]);
+{
+  // write input array into a_qs
+  a_qs := arr;
+  // let quicksort implementation sort a_qs
+  call perm := qs(lo,hi);
+  // write a_qs into output argument
+  arr_sorted := a_qs;
+}
+
+
+procedure bucketSort(lo : int, hi : int) returns (perm: [int]int)
+  modifies a,a_qs; //, b0, b1, b2;
+  // only allow bucketsort to be called from [0..N-1]
+  requires lo == 0;
+  requires hi == N-1;
   // perm is a permutation
   ensures (forall i: int :: lo <= i && i <= hi ==> lo <= perm[i] && perm[i] <= hi);
   ensures (forall k, l: int :: lo <= k && k < l && l <= hi ==> perm[k] != perm[l]);
   // the final array is that permutation of the input array
   ensures (forall i: int :: lo <= i && i <= hi ==> a[i] == old(a)[perm[i]]);
   // array is sorted
-  ensures (forall k, l: int :: lo <= k && k <= l && l <= hi ==> a[k] <= a[l]);
-  // rest of the array is untouched
-  ensures (forall k: int :: k < lo || k > hi ==> a[k] == old(a)[k]);
-{
- // perm is a permutation
-  assume (forall i: int :: lo <= i && i <= hi ==> lo <= perm[i] && perm[i] <= hi);
-  assume (forall k, l: int :: lo <= k && k < l && l <= hi ==> perm[k] != perm[l]);
-  // the final array is that permutation of the input array
-  assume (forall i: int :: lo <= i && i <= hi ==> a[i] == old(a)[perm[i]]);
-  // array is sorted
-  assume (forall k, l: int :: lo <= k && k <= l && l <= hi ==> a[k] <= a[l]);
-  // rest of the array is untouched
-  assume (forall k: int :: k < lo || k > hi ==> a[k] == old(a)[k]);  
-}
-*/
-
-// dummy sort implementation for faster development times
-procedure qs_b0(lo : int, hi : int) returns (perm: [int]int) 
-  modifies b0;
-  requires lo <= hi;
-  
-  ensures (forall i: int :: lo <= i && i <= hi ==> lo <= perm[i] && perm[i] <= hi);
-  ensures (forall k, l: int :: lo <= k && k < l && l <= hi ==> perm[k] != perm[l]);
-  ensures (forall i: int :: lo <= i && i <= hi ==> b0[i] == old(b0)[perm[i]]);
-  ensures (forall k, l: int :: lo <= k && k <= l && l <= hi ==> b0[k] <= b0[l]);
-  ensures (forall k: int :: k < lo || k > hi ==> b0[k] == old(b0)[k]);
-{
-  assume (forall i: int :: lo <= i && i <= hi ==> lo <= perm[i] && perm[i] <= hi);
-  assume (forall k, l: int :: lo <= k && k < l && l <= hi ==> perm[k] != perm[l]);
-  assume (forall i: int :: lo <= i && i <= hi ==> b0[i] == old(b0)[perm[i]]);
-  assume (forall k, l: int :: lo <= k && k <= l && l <= hi ==> b0[k] <= b0[l]);
-  assume (forall k: int :: k < lo || k > hi ==> b0[k] == old(b0)[k]);  
-}
-procedure qs_b1(lo : int, hi : int) returns (perm: [int]int) 
-  modifies b1;
-  requires lo <= hi;
-  
-  ensures (forall i: int :: lo <= i && i <= hi ==> lo <= perm[i] && perm[i] <= hi);
-  ensures (forall k, l: int :: lo <= k && k < l && l <= hi ==> perm[k] != perm[l]);
-  ensures (forall i: int :: lo <= i && i <= hi ==> b1[i] == old(b1)[perm[i]]);
-  ensures (forall k, l: int :: lo <= k && k <= l && l <= hi ==> b1[k] <= b1[l]);
-  ensures (forall k: int :: k < lo || k > hi ==> b1[k] == old(b1)[k]);
-{
-  assume (forall i: int :: lo <= i && i <= hi ==> lo <= perm[i] && perm[i] <= hi);
-  assume (forall k, l: int :: lo <= k && k < l && l <= hi ==> perm[k] != perm[l]);
-  assume (forall i: int :: lo <= i && i <= hi ==> b1[i] == old(b1)[perm[i]]);
-  assume (forall k, l: int :: lo <= k && k <= l && l <= hi ==> b1[k] <= b1[l]);
-  assume (forall k: int :: k < lo || k > hi ==> b1[k] == old(b1)[k]);  
-}
-procedure qs_b2(lo : int, hi : int) returns (perm: [int]int) 
-  modifies b2;
-  requires lo <= hi;
-  
-  ensures (forall i: int :: lo <= i && i <= hi ==> lo <= perm[i] && perm[i] <= hi);
-  ensures (forall k, l: int :: lo <= k && k < l && l <= hi ==> perm[k] != perm[l]);
-  ensures (forall i: int :: lo <= i && i <= hi ==> b2[i] == old(b2)[perm[i]]);
-  ensures (forall k, l: int :: lo <= k && k <= l && l <= hi ==> b2[k] <= b2[l]);
-  ensures (forall k: int :: k < lo || k > hi ==> b2[k] == old(b2)[k]);
-{
-  assume (forall i: int :: lo <= i && i <= hi ==> lo <= perm[i] && perm[i] <= hi);
-  assume (forall k, l: int :: lo <= k && k < l && l <= hi ==> perm[k] != perm[l]);
-  assume (forall i: int :: lo <= i && i <= hi ==> b2[i] == old(b2)[perm[i]]);
-  assume (forall k, l: int :: lo <= k && k <= l && l <= hi ==> b2[k] <= b2[l]);
-  assume (forall k: int :: k < lo || k > hi ==> b2[k] == old(b2)[k]);  
-}
-
-procedure bs() returns (perm: [int]int)
-  modifies a, b0, b1, b2;
-  // perm is a permutation
-  ensures (forall i: int :: 0 <= i && i < N ==> 0 <= perm[i] && perm[i] < N);
-  ensures (forall k, l: int :: 0 <= k && k < l && l < N ==> perm[k] != perm[l]);
-  // the final array is that permutation of the input array
-  ensures (forall i: int :: 0 <= i && i < N ==> a[i] == old(a)[perm[i]]);
-  // array is sorted
-  ensures (forall k, l: int :: 0 <= k && k <= l && l < N ==> a[k] <= a[l]);
+  ensures (forall k, l: int :: lo <= k && k <= l && l <= hi  ==> a[k] <= a[l]);
 {
   
   //buckets' end indices
@@ -281,6 +228,8 @@ procedure bs() returns (perm: [int]int)
   
   //bucket permutations
   var perm0, perm1, perm2 : [int]int;
+
+  var b0, b0_sorted, b1, b1_sorted, b2, b2_sorted: [int]int;
   
   //iterator variables
   var i :int;
@@ -292,11 +241,12 @@ procedure bs() returns (perm: [int]int)
   bound_1 := N;
   bound_2 := 3*N + 1;
   
-  i := 0;
-  while(i < N)
-    invariant (i >= 0 && i <= N);
+  i := lo;
+  while(i <= hi)
+    invariant (i >= lo && i <= hi+1);
     // array 'a' is divided over b0,b1 and b2
-    invariant b0_i+b1_i+b2_i == i;
+    invariant b0_i+b1_i+b2_i == lo+i;
+
     //all buckets contain the correct kind of elements:
     invariant(forall e:int :: (e >= 0 && e < b0_i) ==> (b0[e] < -1*N));
     invariant(forall e:int :: (e >= 0 && e < b1_i) ==> (b1[e] >= -1*N && b1[e] < N));
@@ -323,64 +273,63 @@ procedure bs() returns (perm: [int]int)
     i := i + 1;
   }
   
-  
-  
   // sort first bucket if non-empty
-  if(b0_i > 0) { call perm0 := qs_b0(0, b0_i-1); }
+  if(b0_i > 0) { call b0_sorted, perm0 := quickSort(b0, 0, b0_i-1); }
   // copy back elements from bucket to array
   i := 0;
   while(i < b0_i)
     // copied values are sorted
-    invariant (forall k: int :: 0 <= k && k < i ==> a[k] == b0[k]);
-    invariant (forall k, l: int :: 0 <= k && k <= l && l < i ==> a[k] <= a[l]);
+    invariant (forall k: int :: 0 <= k && k < i ==> a[k+lo] == b0_sorted[k]);
+    invariant (forall k, l: int :: 0 <= k && k <= l && l < i ==> a[k+lo] <= a[l+lo]);
   {
-    a[i] := b0[i];
+    a[i+lo] := b0_sorted[i];
     i := i + 1;
   }
   
   // sort second bucket if non-empty
-  if(b1_i > 0) { call perm1 := qs_b1(0, b1_i-1); }
+  if(b1_i > 0) { call b1_sorted, perm1 := quickSort(b1, 0, b1_i-1); }
   // copy back elements from bucket to array
+
   i := 0;
   while(i < b1_i)
     // preserve info. about first part of array
-    invariant (forall k: int :: 0 <= k && k < b0_i ==> a[k] == b0[k]);
-    invariant (forall k, l: int :: 0 <= k && k <= l && l < b0_i ==> a[k] <= a[l]);
+    invariant (forall k: int :: 0 <= k && k < b0_i ==> a[k+lo] == b0_sorted[k]);
+    invariant (forall k, l: int :: 0 <= k && k <= l && l < b0_i ==> a[k+lo] <= a[l+lo]);
     
     // copied values are sorted
-    invariant (forall k: int :: 0 <= k && k < i ==> a[k+b0_i] == b1[k]);
-    invariant (forall k, l: int :: 0 <= k && k <= l && l < i ==> a[k+b0_i] <= a[l+b0_i]);
+    invariant (forall k: int :: 0 <= k && k < i ==> a[k+lo+b0_i] == b1_sorted[k]);
+    invariant (forall k, l: int :: 0 <= k && k <= l && l < i ==> a[k+lo+b0_i] <= a[l+lo+b0_i]);
       
   {
-    a[i+b0_i] := b1[i];   
+    a[i+lo+b0_i] := b1_sorted[i];   
   }
   
 
   // sort third bucket if non-empty
-  if(b2_i > 0) { call perm2 := qs_b2(0, b2_i-1); }
+  if(b2_i > 0) { call b2_sorted, perm2 := quickSort(b2, 0, b2_i-1); }
   // copy back elements from bucket to array
   i := 0;
   while(i < b2_i)
     // preserve info. about first part of array
-    invariant (forall k: int :: 0 <= k && k < b0_i ==> a[k] == b0[k]);
-    invariant (forall k, l: int :: 0 <= k && k <= l && l < b0_i ==> a[k] <= a[l]);
+    invariant (forall k: int :: 0 <= k && k < b0_i ==> a[k+lo] == b0_sorted[k]);
+    invariant (forall k, l: int :: 0 <= k && k <= l && l < b0_i ==> a[k+lo] <= a[l+lo]);
     
     // preserve info. about second part of array
-    invariant (forall k: int :: 0 <= k && k < b1_i ==> a[k+b0_i] == b1[k]);
-    invariant (forall k, l: int :: 0 <= k && k <= l && l < b1_i ==> a[k+b0_i] <= a[l+b0_i]);
+    invariant (forall k: int :: 0 <= k && k < b1_i ==> a[k+lo+b0_i] == b1_sorted[k]);
+    invariant (forall k, l: int :: 0 <= k && k <= l && l < b1_i ==> a[k+lo+b0_i] <= a[l+lo+b0_i]);
     
     // copied values are sorted
-    invariant (forall k: int :: 0 <= k && k < i ==> a[k+b0_i+b1_i] == b2[k]);
-    invariant (forall k, l: int :: 0 <= k && k <= l && l < i ==> a[k+b0_i+b1_i] <= a[l+b0_i+b1_i]);
+    invariant (forall k: int :: 0 <= k && k < i ==> a[k+lo+b0_i+b1_i] == b2_sorted[k]);
+    invariant (forall k, l: int :: 0 <= k && k <= l && l < i ==> a[k+lo+b0_i+b1_i] <= a[l+lo+b0_i+b1_i]);
   {
-    a[i+b0_i+b1_i] := b2[i];   
+    a[i+lo+b0_i+b1_i] := b2_sorted[i];   
   }
   
   //TODO prove that array is permutation of original
-  assume (forall k: int :: 0 <= k && k < N ==> 0 <= perm[k] && perm[k] < N);
-  assume (forall k, l: int :: 0 <= k && k < l && l < N ==> perm[k] != perm[l]);
+  assume (forall k: int :: lo <= k && k <= hi ==> lo <= perm[k] && perm[k] <= hi);
+  assume (forall k, l: int :: lo <= k && k < l && l <= hi ==> perm[k] != perm[l]);
   // the final array is that permutation of the input array
-  assume (forall k: int :: 0 <= k && k < N ==> a[k] == old(a)[perm[k]]);
+  assume (forall k: int :: lo <= k && k <= hi ==> a[k] == old(a)[perm[k]]);
 
 }
 
